fstar/new/NetworkTypes.fst
@@ -1,0 +1,91 @@
+module NetworkTypes
+
+open Lib.IntTypes
+open Parser
+open Crypto
+
+noeq type kdf_label = {
+  length: uint16;
+  label: blbytes ({min=7; max=255});
+  context: blbytes ({min=0; max=(pow2 32)-1});
+}
+
+val ps_kdf_label: parser_serializer kdf_label
+let ps_kdf_label =
+  isomorphism
+    kdf_label
+    (
+      _ <-- ps_u16;
+      _ <-- ps_bytes _;
+      ps_bytes _
+    )
+    (fun (|length, (|label, context|)|) -> {length=length; label=label; context=context;})
+    (fun x -> (|x.length, (|x.label, x.context|)|))
+
+noeq type hpke_ciphertext = {
+  kem_output: blbytes ({min=0; max=(pow2 16)-1});
+  ciphertext: blbytes ({min=0; max=(pow2 16)-1});
+}
+
+val ps_hpke_ciphertext: parser_serializer hpke_ciphertext
+let ps_hpke_ciphertext =
+  isomorphism
+    hpke_ciphertext
+    (
+      _ <-- ps_bytes _;
+      ps_bytes _
+    )
+    (fun (|kem_output, ciphertext|) -> {kem_output=kem_output; ciphertext=ciphertext;})
+    (fun x -> (|x.kem_output, x.ciphertext|))
+
+
+noeq type update_path_node (cs:ciphersuite) = {
+  public_key: hpke_public_key cs;
+  encrypted_path_secret: blseq hpke_ciphertext ps_hpke_ciphertext ({min=0; max=(pow2 32)-1});
+}
+
+val ps_update_path_node: cs:ciphersuite -> parser_serializer (update_path_node cs)
+let ps_update_path_node cs =
+  assume (1 <= hpke_public_key_length cs); //TODO
+  isomorphism
+    (update_path_node cs)
+    (
+      _ <-- ps_lbytes (hpke_public_key_length cs);
+      ps_seq _ ps_hpke_ciphertext
+    )
+    (fun (|public_key, encrypted_path_secret|) -> {public_key=public_key; encrypted_path_secret=encrypted_path_secret;})
+    (fun x -> (|x.public_key, x.encrypted_path_secret|))
+
+noeq type key_package (cs:ciphersuite) = {
+  //TODO
+  public_key: hpke_public_key cs;
+  //TODO
+}
+
+val ps_key_package: cs:ciphersuite -> parser_serializer (key_package cs)
+let ps_key_package cs =
+  assume (1 <= hpke_public_key_length cs); //TODO
+  isomorphism
+    (key_package cs)
+    (
+      ps_lbytes (hpke_public_key_length cs)
+    )
+    (fun public_key -> {public_key=public_key})
+    (fun x -> x.public_key)
+
+//TODO: this type will be converted to a `path` for TreeSync / TreeKEM. Should we parse a `path` directly and hide this internal record?
+noeq type update_path (cs:ciphersuite) = {
+  leaf_key_package: key_package cs;
+  nodes: blseq (update_path_node cs) (ps_update_path_node cs) ({min=0; max=(pow2 32)-1});
+}
+
+val ps_update_path: cs:ciphersuite -> parser_serializer (update_path cs)
+let ps_update_path cs =
+  isomorphism
+    (update_path cs)
+    (
+      _ <-- ps_key_package cs;
+      ps_seq _ (ps_update_path_node cs)
+    )
+    (fun (|leaf_key_package, nodes|) -> {leaf_key_package=leaf_key_package; nodes=nodes})
+    (fun x -> (|x.leaf_key_package, x.nodes|))
